src/Bedrock/Field/FieldExtensions/GenericQuadraticFeval.v
@@ -1,113 +1,61 @@
 (** * Generic algebraic identities for quadratic extensions.
-
-    Proves ring-theoretic identities about the abstract quadratic
-    extension operations (from QuadraticExtensionsAbstract.v) that
-    hold for any commutative base field.
-
-    These identities are the building blocks of per-curve feval chains.
-    Each curve's feval file instantiates these with specific beta/xi
-    values and bridges to its pairing spec.
-
-    Key lemmas:
-    - [qe_mul_self_alt]       : qe_mul x x has 2ab in imaginary part
-    - [qe_sub_sub_eq_sub_add] : (x-y)-z = x-(y+z) componentwise
-    - [qe_add_sub_eq_sub_add] : (x-y)+z = (x+z)-y componentwise
-    - [qe_mul_comm]           : qe_mul x y = qe_mul y x
-
     Requires: a stdlib [ring_theory] for the base field. *)
 
+Require Import Crypto.Bedrock.Specs.AbstractField.
 Require Import Crypto.Bedrock.Field.FieldExtensions.Theory.QuadraticExtensionsAbstract.
+From Stdlib Require Import Ring_theory Ring.
 
 Section QuadraticFeval.
-
-  Context {F : Type}.
-  Variable Fzero Fone : F.
-  Variable Fopp : F -> F.
-  Variable Finv : F -> F.
-  Variable Fadd Fsub Fmul : F -> F -> F.
-  Variable Fdiv : F -> F -> F.
+  Context {F : Type} {fp : FieldParameters F}.
   Variable nonresidue : F.
 
-  Hypothesis Frt : ring_theory Fzero Fone Fadd Fmul Fsub Fopp (@eq F).
+  Hypothesis Frt : ring_theory (@Fzero _ fp) (@Fone _ fp)
+    (@Fadd _ fp) (@Fmul _ fp) (@Fsub _ fp) (@Fopp _ fp) (@eq F).
   Add Ring base_ring : Frt.
 
   Local Notation QE := (F * F)%type.
-  Local Notation qe_add := (qe_add Fadd).
-  Local Notation qe_sub := (qe_sub Fsub).
-  Local Notation qe_opp := (qe_opp Fopp).
-  Local Notation qe_mul := (qe_mul Fadd Fmul nonresidue).
-
-  (* ================================================================ *)
-  (* Sub-associativity and grouping (componentwise ring algebra)       *)
-  (* ================================================================ *)
 
   Lemma qe_sub_sub_eq_sub_add : forall x y z : QE,
-    qe_sub (qe_sub x y) z = qe_sub x (qe_add y z).
+    @qe_sub _ fp (@qe_sub _ fp x y) z =
+    @qe_sub _ fp x (@qe_add _ fp y z).
   Proof.
     intros [x0 x1] [y0 y1] [z0 z1].
-    unfold QuadraticExtensionsAbstract.qe_sub, QuadraticExtensionsAbstract.qe_add;
-      simpl fst; simpl snd.
-    f_equal; ring.
+    unfold qe_sub, qe_add; simpl fst; simpl snd. f_equal; ring.
   Qed.
 
   Lemma qe_add_sub_eq_sub_add : forall x y z : QE,
-    qe_add (qe_sub x y) z = qe_sub (qe_add x z) y.
+    @qe_add _ fp (@qe_sub _ fp x y) z =
+    @qe_sub _ fp (@qe_add _ fp x z) y.
   Proof.
     intros [x0 x1] [y0 y1] [z0 z1].
-    unfold QuadraticExtensionsAbstract.qe_add, QuadraticExtensionsAbstract.qe_sub;
-      simpl fst; simpl snd.
-    f_equal; ring.
+    unfold qe_add, qe_sub; simpl fst; simpl snd. f_equal; ring.
   Qed.
-
-  (* ================================================================ *)
-  (* Multiplication commutativity                                      *)
-  (* ================================================================ *)
 
   Lemma qe_mul_comm : forall x y : QE,
-    qe_mul x y = qe_mul y x.
+    @qe_mul _ fp nonresidue x y = @qe_mul _ fp nonresidue y x.
   Proof.
     intros [a0 a1] [b0 b1].
-    unfold QuadraticExtensionsAbstract.qe_mul; simpl fst; simpl snd.
-    f_equal; ring.
+    unfold qe_mul; simpl fst; simpl snd. f_equal; ring.
   Qed.
 
-  (* ================================================================ *)
-  (* mul(x,x) alternative form (for squaring optimization)             *)
-  (* ================================================================ *)
-
-  (** qe_mul x x computes:
-        re = Fmul a a + nr * (Fmul b b)
-        im = Fmul a b + Fmul b a = 2 * Fmul a b  (by commutativity)
-
-      The bedrock2 squaring function uses this "2ab" form for im,
-      and "a² + nr*b²" for re.  This lemma shows qe_mul x x has
-      the same form. *)
   Lemma qe_mul_self_alt : forall x : QE,
-    qe_mul x x =
+    @qe_mul _ fp nonresidue x x =
     (Fadd (Fmul (fst x) (fst x)) (Fmul nonresidue (Fmul (snd x) (snd x))),
      Fadd (Fmul (fst x) (snd x)) (Fmul (fst x) (snd x))).
   Proof.
-    intros [a0 a1].
-    unfold QuadraticExtensionsAbstract.qe_mul; simpl fst; simpl snd.
-    f_equal; ring.
+    intros [a0 a1]. unfold qe_mul; simpl fst; simpl snd. f_equal; ring.
   Qed.
 
-  (* ================================================================ *)
-  (* Karatsuba cross-term: (a+b)² - a² - b² = 2ab                    *)
-  (* ================================================================ *)
-
   Lemma qe_karatsuba_cross_term : forall a b : QE,
-    qe_sub (qe_sub (qe_mul (qe_add a b) (qe_add a b))
-                    (qe_mul a a))
-           (qe_mul b b) =
-    qe_add (qe_mul a b) (qe_mul a b).
+    @qe_sub _ fp
+      (@qe_sub _ fp
+        (@qe_mul _ fp nonresidue (@qe_add _ fp a b) (@qe_add _ fp a b))
+        (@qe_mul _ fp nonresidue a a))
+      (@qe_mul _ fp nonresidue b b) =
+    @qe_add _ fp (@qe_mul _ fp nonresidue a b) (@qe_mul _ fp nonresidue a b).
   Proof.
     intros [a0 a1] [b0 b1].
-    unfold QuadraticExtensionsAbstract.qe_mul,
-           QuadraticExtensionsAbstract.qe_add,
-           QuadraticExtensionsAbstract.qe_sub;
-      simpl fst; simpl snd.
-    f_equal; ring.
+    unfold qe_mul, qe_add, qe_sub; simpl fst; simpl snd. f_equal; ring.
   Qed.
 
 End QuadraticFeval.
